---
title: "DATA 605 Week 14"
author: "Mike Silva"
date: "April 27, 2019"
output: html_document
---

## $f(x) = \frac{1}{(1-x)}$

| Derivative                   | Solved at zero |
|------------------------------|----------------|
| $f(x) = \frac{1}{(1-x)}$     | $f(0) = 1$     |
| $f'(x) = \frac{1}{(1-x)^2}$  | $f'(0) = 1$    |
| $f''(x) = \frac{2}{(1-x)^3}$ | $f''(0) = 2$   |
| $f'''(x) = \frac{6}{(1-x)^4}$| $f'''(0) = 6$  |

$1 + \frac{1}{1!} x^1 + \frac{2}{2!} x^2 + \frac{6}{3!}x^3 ...$

Which simplies and generalizes to:

$$1 + x +x^2 + x^3 + ... + x^n$$

Expressed as a summation:

$$\sum_{n=0}^{\infty} x^n$$

This function is undefined at x=1.

## $f(x) = e^x$

| Derivative     | Solved at zero |
|----------------|----------------|
| $f(x) = e^x$   | $f(0) = 1$     |
| $f'(x) = e^x$  | $f'(0) = 1$    |
| $f''(x) = e^x$ | $f''(0) = 1$   |
| $f'''(x) = e^x$| $f'''(0) = 1$  |

$1 + \frac{1}{1!} x^1 + \frac{1}{2!} x^2 + \frac{1}{3!}x^3...$

Which simplies and generalizes to:

$$1 + x +x^2 + x^3 + ... + x^n$$


Expressed as a summation:

$$\sum_{n=0}^{\infty} \frac{x^n}{n!}$$

## $f(x) = ln(1+x)$

| Derivative                  | Solved at zero |
|-----------------------------|----------------|
| $f(x) = ln(1+x)$            | $f(0) = 0$     |
| $f'(x) = \frac{1}{(1+x)}$   | $f'(0) = 1$    |
| $f''(x) = -\frac{2}{(1+x)}$ | $f''(0) = -1$  |
| $f'''(x) = \frac{6}{(1+x)}$ | $f'''(0) = 2$  |

This is similar to the first equation

$0 + \frac{1}{1!} x^1 - \frac{1}{2!} x^2 + \frac{2}{3!}x^3 ...$

Or

$x - \frac{1}{2} x^2 + \frac{1}{4}x^3 ...$

The alternating plus minus can be described with 

$(-1)^{n+1}$

So the generalized form is 

$x - \frac{1}{2} x^2 + \frac{1}{4}x^3 ... (-1)^{n+1}\frac{1}{n}x^n$

Expressed as a summation:

$$\sum_{n=0}^{\infty} (-1)^{n+1}\frac{1}{n}x^n$$